src/Crypto/RSAEncryption.dfy
@@ -1,3 +1,4 @@
+
 include "../StandardLibrary/StandardLibrary.dfy"
 
 //This code must be reviewed, see #18
@@ -43,23 +44,18 @@ module {:extern "RSAEncryption"} RSAEncryption {
 
         // TODO: below should return an option if anything throws.
         static method {:extern "RSAKeygen"} RSAKeygen(bits : RSABitLength, padding: RSAPaddingMode) returns (ek : seq<uint8>, dk : seq<uint8>)
-            ensures RSAWfEK(bits, padding, ek)
-            ensures RSAWfDK(bits, padding, dk)
-            ensures IsRSAKeypair(bits, padding, ek, dk)
-
-        static function method {:extern "RSADecrypt"} RSADecrypt(bits : RSABitLength, padding : RSAPaddingMode, dk : seq<uint8>, c : seq<uint8>) : Option<seq<uint8>>
-            // requires RSAWfCtx(bits, padding, c) -- there should be a runtime way to establish this. or maybe not?
-            requires RSAWfDK(bits, padding, dk) // similarly how should I validate the key is well formed
-
-        static method {:extern "RSAEncrypt"} RSAEncrypt(bits : RSABitLength, padding: RSAPaddingMode, ek : seq<uint8>, msg : seq<uint8>) returns (c : Option<seq<uint8>>)
-            requires RSAWfEK(bits, padding, ek) // todo: be able to validate this at runtime
-            ensures c.Some? ==> RSAWfCtx(bits,padding, c.get)
-            ensures c.Some? ==> forall dk :: IsRSAKeypair(bits,padding,ek, dk) ==> RSAWfDK(bits,padding,dk) ==> RSADecrypt(bits, padding, dk, c.get) == Some(msg)
-        
-        static method {:extern "StringToPEM"} StringToPEM(privatePEM: string, publicPEM: string) returns (ek : seq<uint8>, dk : seq<uint8>)
             ensures RSAWfEK(padding, ek)
             ensures RSAWfDK(padding, dk)
             ensures IsRSAKeypair(padding, ek, dk)
+
+        static function method {:extern "RSADecrypt"} RSADecrypt(padding : RSAPaddingMode, dk : seq<uint8>, c : seq<uint8>) : Result<seq<uint8>>
+            // requires RSAWfCtx(padding, c) -- there should be a runtime way to establish this. or maybe not?
+
+        static method {:extern "RSAEncrypt"} RSAEncrypt(padding: RSAPaddingMode, ek : seq<uint8>, msg : seq<uint8>) returns (res : Result<seq<uint8>>)
+            ensures res.Success? ==> RSAWfCtx(padding, res.value)
+            ensures res.Success? ==> forall dk :: IsRSAKeypair(padding, ek, dk) ==> RSAWfDK(padding, dk) ==> RSADecrypt(padding, dk, res.value) == Success(msg)
+
+        static method {:extern "StringToPEM"} StringToPEM(privatePEM: string, publicPEM: string) returns (ek : seq<uint8>, dk : seq<uint8>)
     }
 
 }
